@prefix : <http://www.semanticweb.org/ontologies/2024/11/InvestmentFinanceOnto#> .
@prefix owl: <http://www.w3.org/2002/07/owl#> .
@prefix rdf: <http://www.w3.org/1999/02/22-rdf-syntax-ns#> .
@prefix rdfs: <http://www.w3.org/2000/01/rdf-schema#> .

# ========================================
# PORTFOLIO CLASSES
# ========================================

:Investor rdf:type owl:Class ;
    rdfs:comment "Individual or entity that allocates capital with the expectation of a future financial return" .

:Portfolio rdf:type owl:Class ;
    rdfs:comment "A collection of financial investments like stocks, bonds, commodities, cash, and cash equivalents" .


# ========================================
# PORTFOLIO PROPERTIES
# ========================================

:ownedBy rdf:type owl:ObjectProperty ;
    rdfs:domain :Portfolio ;
    rdfs:range :Investor ;
    rdfs:comment "Identifies the owner of the investment portfolio" .

:holds rdf:type owl:ObjectProperty ;
    rdfs:domain :Portfolio ;
    rdfs:range :InvestmentInstrument ;
    rdfs:comment "Indicates that a portfolio contains a specific investment instrument" .
